Complete revised version of renumber.

sepcomp/backend/Renumberproof_sepcomp.v
@@ -54,7 +54,6 @@ Lemma functions_translated:
   forall v f,
   Genv.find_funct ge v = Some f ->
   exists tf, Genv.find_funct tge v = Some tf /\ (match_fundef f tf).
-(*  Genv.find_funct tge v = Some (transf_fundef f).*)
 Proof.
   generalize (find_funct_transf' _ _ TRANSF).
   intros H1 v f. specialize (H1 v f).
@@ -182,29 +181,6 @@ Proof.
   unfold successors_map. rewrite PTree.gmap1. rewrite H. auto. 
 Qed.
 
-
-(*
-Inductive match_transl_frames: RTL.stackframe -> RTL.stackframe -> Prop :=
-  | match_transl_frames_intro: forall res f sp pc rs
-        (REACH: reach f pc),
-      match_transl_frames (Stackframe res f sp pc rs)
-                   (Stackframe res (transf_function f) sp (renum_pc (pnum f) pc) rs).
-
-Inductive match_identical_frames: RTL.stackframe -> RTL.stackframe -> Prop :=
-  | match_identical_frames_intro: forall res f sp pc rs,
-      match_identical_frames (Stackframe res f sp pc rs)
-                   (Stackframe res f sp pc rs).
-
-Inductive match_frames: RTL.stackframe -> RTL.stackframe -> Prop :=
-| match_frames_transl: forall fr1 fr2
-                              (MATCHTR: match_transl_frames fr1 fr2),
-                         match_frames fr1 fr2
-| match_frames_identical: forall fr1 fr2
-                                 (MATCHID: match_identical_frames fr1 fr2),
-                            match_frames fr1 fr2
-.
-*)
-
 Inductive match_frames: RTL.stackframe -> RTL.stackframe -> Prop :=
   | match_transl_frames_intro': forall res f sp pc rs
         (REACH: reach f pc),
@@ -215,85 +191,73 @@ Inductive match_frames: RTL.stackframe -> RTL.stackframe -> Prop :=
                    (Stackframe res f sp pc rs)
 .
 
-
-Inductive match_transl_states: RTL.state -> RTL.state -> Prop :=
-  | match_transl_regular_states: forall stk f sp pc rs m stk'
-        (STACKS: list_forall2 match_frames stk stk')
-        (REACH: reach f pc),
-      match_transl_states (State stk f sp pc rs m)
-                   (State stk' (transf_function f) sp (renum_pc (pnum f) pc) rs m)
-  | match_transl_callstates: forall stk f f' args m stk'
-        (FD: match_fundef f f')
-        (STACKS: list_forall2 match_frames stk stk'),
-      match_transl_states (Callstate stk f args m)
-                   (Callstate stk' f' args m)
-  | match_transl_returnstates: forall stk v m stk'
-        (STACKS: list_forall2 match_frames stk stk'),
-      match_transl_states (Returnstate stk v m)
-                   (Returnstate stk' v m).
-
-Inductive match_identical_states: RTL.state -> RTL.state -> Prop :=
-  | match_identical_regular_states: forall stk f sp pc rs m stk'
-        (STACKS: list_forall2 match_frames stk stk'),
-      match_identical_states (State stk f sp pc rs m)
-                   (State stk' f sp pc rs m)
-.
-
 Inductive match_states: RTL.state -> RTL.state -> Prop :=
-| match_states_transl: forall st1 st2
-                               (MSTATE: match_transl_states st1 st2),
-                          match_states st1 st2
-| match_states_identical: forall st1 st2
-                               (MSTATE: match_identical_states st1 st2),
-                          match_states st1 st2
-.
-
-(* original
-Inductive match_states: RTL.state -> RTL.state -> Prop :=
-  | match_regular_states: forall stk f sp pc rs m stk'
+| match_transl_regular_states: forall stk f sp pc rs m stk'
         (STACKS: list_forall2 match_frames stk stk')
         (REACH: reach f pc),
       match_states (State stk f sp pc rs m)
                    (State stk' (transf_function f) sp (renum_pc (pnum f) pc) rs m)
-  | match_callstates: forall stk f args m stk'
+| match_transl_callstates: forall stk f f' args m stk'
+        (FD: match_fundef f f')
         (STACKS: list_forall2 match_frames stk stk'),
       match_states (Callstate stk f args m)
-                   (Callstate stk' (transf_fundef f) args m)
-  | match_returnstates: forall stk v m stk'
+                   (Callstate stk' f' args m)
+| match_transl_returnstates: forall stk v m stk'
         (STACKS: list_forall2 match_frames stk stk'),
       match_states (Returnstate stk v m)
-                   (Returnstate stk' v m).
-*)
-Lemma step_simulation_transl:
+                   (Returnstate stk' v m)
+| match_identical_regular_states: forall stk f sp pc rs m stk'
+        (STACKS: list_forall2 match_frames stk stk'),
+      match_states (State stk f sp pc rs m)
+                   (State stk' f sp pc rs m)
+.
+
+Lemma step_simulation:
   forall S1 t S2, RTL.step ge S1 t S2 ->
-  forall S1', match_transl_states S1 S1' ->
+  forall S1', match_states S1 S1' ->
   exists S2', RTL.step tge S1' t S2' /\ match_states S2 S2'.
 Proof.
   induction 1; intros S1' MS; inv MS; try TR_AT.
 (* nop *)
   econstructor; split. eapply exec_Inop; eauto.
-  constructor.
-  constructor; auto. eapply reach_succ; eauto. simpl; auto. 
+  constructor; auto. eapply reach_succ; eauto. simpl; auto.
+(* nop2 *)
+  econstructor; split. eapply exec_Inop; eauto.
+  constructor; auto.
 (* op *)
   econstructor; split.
   eapply exec_Iop; eauto.
   instantiate (1 := v). rewrite <- H0. apply eval_operation_preserved. exact symbols_preserved.
-  constructor.
   constructor; auto. eapply reach_succ; eauto. simpl; auto.
+(* op2 *)
+  econstructor; split.
+  eapply exec_Iop; eauto.
+  instantiate (1 := v). rewrite <- H0. apply eval_operation_preserved. exact symbols_preserved.
+  constructor; auto.
 (* load *)
   econstructor; split.
   assert (eval_addressing tge sp addr rs ## args = Some a).
   rewrite <- H0. apply eval_addressing_preserved. exact symbols_preserved. 
   eapply exec_Iload; eauto.
-  constructor.
   constructor; auto. eapply reach_succ; eauto. simpl; auto.
+(* load2 *)
+  econstructor; split.
+  assert (eval_addressing tge sp addr rs ## args = Some a).
+  rewrite <- H0. apply eval_addressing_preserved. exact symbols_preserved. 
+  eapply exec_Iload; eauto.
+  constructor; auto.
 (* store *)
   econstructor; split.
   assert (eval_addressing tge sp addr rs ## args = Some a).
   rewrite <- H0. apply eval_addressing_preserved. exact symbols_preserved. 
   eapply exec_Istore; eauto.
-  constructor.
   constructor; auto. eapply reach_succ; eauto. simpl; auto.
+(* store2 *)
+  econstructor; split.
+  assert (eval_addressing tge sp addr rs ## args = Some a).
+  rewrite <- H0. apply eval_addressing_preserved. exact symbols_preserved. 
+  eapply exec_Istore; eauto.
+  constructor; auto.
 (* call *)
   exploit find_function_translated; eauto.
   intros Htfd. destruct Htfd as [tfd [findtfd matchtfd]].
@@ -301,7 +265,15 @@ Proof.
   eapply exec_Icall with (fd := tfd); eauto.
   inv matchtfd; auto.
     apply sig_preserved.
-  constructor. constructor; auto. constructor; auto. constructor. eapply reach_succ; eauto. simpl; auto.
+  constructor; auto. constructor; auto. constructor. eapply reach_succ; eauto. simpl; auto.
+(* call2 *)
+  exploit find_function_translated; eauto.
+  intros Htfd. destruct Htfd as [tfd [findtfd matchtfd]].
+  econstructor; split.
+  eapply exec_Icall with (fd := tfd); eauto.
+  inv matchtfd; auto.
+    apply sig_preserved.
+  constructor; auto. constructor; auto. constructor.
 (* tailcall *)
   exploit find_function_translated; eauto.
   intros Htfd. destruct Htfd as [tfd [findtfd matchtfd]].
@@ -309,38 +281,63 @@ Proof.
   eapply exec_Itailcall with (fd := tfd); eauto.
   inv matchtfd; auto.
     apply sig_preserved.
-  constructor. constructor; auto.
+  constructor; auto.
+(* tailcall2 *)
+  exploit find_function_translated; eauto.
+  intros Htfd. destruct Htfd as [tfd [findtfd matchtfd]].
+  econstructor; split.
+  eapply exec_Itailcall with (fd := tfd); eauto.
+  inv matchtfd; auto.
+    apply sig_preserved.
+  constructor; auto.
 (* builtin *)
   econstructor; split.
   eapply exec_Ibuiltin; eauto.
     eapply external_call_symbols_preserved; eauto.
     exact symbols_preserved. exact varinfo_preserved.
-  constructor; auto. constructor; auto. eapply reach_succ; eauto. simpl; auto.
+  constructor; auto. eapply reach_succ; eauto. simpl; auto.
+(* builtin2 *)
+  econstructor; split.
+  eapply exec_Ibuiltin; eauto.
+    eapply external_call_symbols_preserved; eauto.
+    exact symbols_preserved. exact varinfo_preserved.
+  constructor; auto.
 (* cond *)
   econstructor; split.
   eapply exec_Icond; eauto. 
   replace (if b then renum_pc (pnum f) ifso else renum_pc (pnum f) ifnot)
      with (renum_pc (pnum f) (if b then ifso else ifnot)).
-  constructor; auto. constructor; auto. eapply reach_succ; eauto. simpl. destruct b; auto. 
+  constructor; auto. eapply reach_succ; eauto. simpl. destruct b; auto. 
   destruct b; auto.
+(* cond2 *)
+  econstructor; split.
+  eapply exec_Icond; eauto.
+  constructor; auto.
 (* jumptbl *)
   econstructor; split.
   eapply exec_Ijumptable; eauto. rewrite list_nth_z_map. rewrite H1. simpl; eauto. 
-  constructor; auto. constructor; auto. eapply reach_succ; eauto. simpl. eapply list_nth_z_in; eauto. 
+  constructor; auto. eapply reach_succ; eauto. simpl. eapply list_nth_z_in; eauto.
+(* jumptbl2 *)
+  econstructor; split.
+  eapply exec_Ijumptable; eauto.
+  constructor; auto.
 (* return *)
   econstructor; split.
   eapply exec_Ireturn; eauto. 
-  constructor; auto. constructor; auto.
+  constructor; auto.
+(* return2 *)
+  econstructor; split.
+  eapply exec_Ireturn; eauto. 
+  constructor; auto.
 (* internal function *)
   inv FD.
   simpl. econstructor; split.
   eapply exec_function_internal; eauto. 
-  constructor; auto.
   constructor; auto. unfold reach. constructor.
-
+(* internal function2 *)
   simpl. econstructor; split.
   eapply exec_function_internal; eauto.
-  apply match_states_identical. constructor; auto.
+  constructor; auto.
 (* external function *)
   inv FD.
   econstructor; split.
@@ -348,104 +345,22 @@ Proof.
     eapply external_call_symbols_preserved; eauto.
     exact symbols_preserved. exact varinfo_preserved.
   constructor; auto.
-  constructor; auto.
-
+(* external function2 *)
   econstructor; split.
   eapply exec_function_external; eauto.
     eapply external_call_symbols_preserved; eauto.
     exact symbols_preserved. exact varinfo_preserved.
-  constructor; auto.
   constructor; auto.
 (* return *)
   inv STACKS. inv H1.
   econstructor; split. 
   eapply exec_return; eauto. 
   constructor; auto.
-  constructor; auto.
-
+(* return2 *)
   econstructor; split. 
   eapply exec_return; eauto.
-  apply match_states_identical.
   constructor; auto.
 Qed.
-
-Lemma step_simulation_identical:
-  forall S1 t S2, RTL.step ge S1 t S2 ->
-  forall S1', match_identical_states S1 S1' ->
-  exists S2', RTL.step tge S1' t S2' /\ match_states S2 S2'.
-Proof.
-  induction 1; intros S1' MS; inv MS; try TR_AT.
-(* nop *)
-  econstructor; split. eapply exec_Inop; eauto.
-  apply match_states_identical.
-  constructor; auto.
-(* op *)
-  econstructor; split.
-  eapply exec_Iop; eauto.
-  instantiate (1 := v). rewrite <- H0. apply eval_operation_preserved. exact symbols_preserved.
-  apply match_states_identical.
-  constructor; auto.
-(* load *)
-  econstructor; split.
-  assert (eval_addressing tge sp addr rs ## args = Some a).
-  rewrite <- H0. apply eval_addressing_preserved. exact symbols_preserved. 
-  eapply exec_Iload; eauto.
-  apply match_states_identical.
-  constructor; auto.
-(* store *)
-  econstructor; split.
-  assert (eval_addressing tge sp addr rs ## args = Some a).
-  rewrite <- H0. apply eval_addressing_preserved. exact symbols_preserved. 
-  eapply exec_Istore; eauto.
-  apply match_states_identical.
-  constructor; auto.
-(* call *)
-  exploit find_function_translated; eauto.
-  intros Htfd. destruct Htfd as [tfd [findtfd matchtfd]].
-  econstructor; split.
-  eapply exec_Icall with (fd := tfd); eauto.
-  inv matchtfd; auto.
-    apply sig_preserved.
-  constructor. constructor; auto. constructor; auto. constructor.
-(* tailcall *)
-  exploit find_function_translated; eauto.
-  intros Htfd. destruct Htfd as [tfd [findtfd matchtfd]].
-  econstructor; split.
-  eapply exec_Itailcall with (fd := tfd); eauto.
-  inv matchtfd; auto.
-    apply sig_preserved.
-  constructor. constructor; auto.
-(* builtin *)
-  econstructor; split.
-  eapply exec_Ibuiltin; eauto.
-    eapply external_call_symbols_preserved; eauto.
-    exact symbols_preserved. exact varinfo_preserved.
-  apply match_states_identical.
-  constructor; auto.
-(* cond *)
-  econstructor; split.
-  eapply exec_Icond; eauto.
-  apply match_states_identical. constructor; auto.
-(* jumptbl *)
-  econstructor; split.
-  eapply exec_Ijumptable; eauto.
-  apply match_states_identical. constructor; auto.
-(* return *)
-  econstructor; split.
-  eapply exec_Ireturn; eauto. 
-  apply match_states_transl. constructor; auto.
-Qed.
-
-Lemma step_simulation:
-  forall S1 t S2, RTL.step ge S1 t S2 ->
-  forall S1', match_states S1 S1' ->
-  exists S2', RTL.step tge S1' t S2' /\ match_states S2 S2'.
-Proof.
-  intros. inv H0.
-  - eapply step_simulation_transl; eauto.
-  - eapply step_simulation_identical; eauto.
-Qed.
-
 
 Lemma transf_initial_states:
   forall S1, RTL.initial_state prog S1 ->
@@ -463,17 +378,13 @@ Proof.
     eauto.    
     inv matchtf; auto.
     rewrite <- H3; apply sig_preserved.
-    
-  constructor. constructor.
-  auto.
-  constructor.
+  constructor; auto. constructor.
 Qed.
 
 Lemma transf_final_states:
   forall S1 S2 r, match_states S1 S2 -> RTL.final_state S1 r -> RTL.final_state S2 r.
 Proof.
-  intros. inv H0. inv H; inv MSTATE.
-  inv STACKS. constructor.
+  intros. inv H0. inv H. inv STACKS. constructor.
 Qed.
 
 Theorem transf_program_correct:
